checker/checkTrace.mli
@@ -2,3 +2,6 @@
  * and the initial clauses of a resolution proof. *)
 val assumptions : Model.t -> (int, MTypes.lit) Hashtbl.t ->
   Genlex.token Stream.t -> MTypes.clause list
+
+val assumptions_sdrup : Model.t -> (int, MTypes.lit) Hashtbl.t ->
+  char Stream.t -> MTypes.clause list
