checker/model.ml
@@ -3,6 +3,7 @@ module MT = MTypes
 module H = Hashtbl
 module A = DynArray
 module C = Checker
+module Sol = SolCheck
 
 type ident = MT.ident
 
@@ -15,13 +16,19 @@ type ident_kind =
 | IdCon  (* Constraint (with associated checker) *)
 | IdProp (* Proposition *)
 
+type constraint_info = {
+  name : ident ;
+  mutable checkers : C.t list ;
+  mutable sol_check : Sol.t option ;
+}
 type model = {
   (* Symbol table. *)
   symbols : (ident, ident_kind*int) Hashtbl.t;
 
   bvars : ident A.t ;
   ivars : (ident * ((int*int) option)) A.t ;
-  constraints : (ident * C.t) A.t;
+  (* constraints : (ident * C.t) A.t; *)
+  constraints : constraint_info A.t;
   vprops : (ident * MT.lit) A.t
 }
 
@@ -52,10 +59,35 @@ let add_lit model ident prop =
   Hashtbl.add model.symbols ident (IdProp, idx) ;
   A.add model.vprops (ident, prop)
 
+let constraint_id model ident =
+  try
+    let (kind, idx) = Hashtbl.find model.symbols ident in
+    match kind with
+    | IdCon -> idx
+    | _ -> error (Format.sprintf "Error:  Identifier %s not a constraint." ident)
+  with Not_found ->
+    let idx = A.length model.constraints
+    and elt = {
+      name = ident ;
+      checkers = [] ;
+      sol_check = None
+    } in
+    begin
+      Hashtbl.add model.symbols ident (IdCon, idx) ;
+      A.add model.constraints elt ;
+      idx
+    end
+    
+let get_constraint_info model ident =
+  A.get model.constraints (constraint_id model ident)
+
 let add_checker model ident checker =
-  let idx = A.length model.constraints in
-  Hashtbl.add model.symbols ident (IdCon, idx) ;
-  A.add model.constraints (ident, checker)
+  let elt = get_constraint_info model ident in
+  elt.checkers <- checker :: elt.checkers
+
+let add_sol_check model ident sol_check =
+  let elt = get_constraint_info model ident in
+  elt.sol_check <- Some sol_check
 
 let get_ivar (model : t) ident =
   try
@@ -91,6 +123,10 @@ let get_lit (model : t) ident =
 let lits_iteri f model = A.iteri (fun i (id, lit) -> f i id lit) model.vprops
 
 let get_checker model ident =
+  match (get_constraint_info model ident).checkers with
+  | [] -> error (Format.sprintf "Error: No checker registered for %s." ident)
+  | (x :: xs) -> x
+  (*
   try
     let (kind, idx) = Hashtbl.find model.symbols ident in
     match kind with
@@ -98,9 +134,16 @@ let get_checker model ident =
     | _ -> failwith (Format.sprintf "Error: symbol %s not a constraint." ident)
   with Not_found ->
     failwith (Format.sprintf "Error: symbol not found - %s." ident)
+  *)
 
 let get_all_checkers model =
-  A.fold_left (fun cs (_, check) -> check :: cs) [] model.constraints
+  A.fold_left (fun cs elt -> List.append elt.checkers cs) [] model.constraints
+
+let get_sol_checkers model =
+  A.fold_left (fun cs elt ->
+    match elt.sol_check with
+    | Some check -> check :: cs
+    | None -> (Sol.fail elt.name) :: cs) [] model.constraints
 
 let string_of_vprop model = function
 | MT.ILe (x, k) -> (ivar_name model x) ^ "<=" ^ (string_of_int k)
