checker/registry.ml
@@ -1,8 +1,11 @@
 (* Registry of checkers for constraint classes. *)
+module MT = MTypes
 module H = Hashtbl
 module C = Checker
+module Sol = SolCheck
 
 let registry = H.create 17
+let sol_registry = H.create 17
 
 let fmt = Format.std_formatter
 let err_fmt = Format.err_formatter
@@ -23,10 +26,21 @@ let null_checker model =
       }
     end
 
-(* Register a new checker kind. *)
-let add ident checker = H.add registry ident checker
+let null_sol_checker model =
+  fun tokens ->
+    begin
+      drop_args tokens;
+      {
+        Sol.repr = "null-solcheck" ;
+        Sol.check = (fun _ -> false)
+      }
+    end
+
+let add = H.add registry
+let add_sol = H.add sol_registry
 
 (* Find the checker-constructor for the given class. *)
+(*
 let find ident =
   try
     H.find registry ident
@@ -38,4 +52,19 @@ let find ident =
         add ident null_checker ;
         null_checker
       end
+*)
+let find_impl tbl default warn ident =
+  try
+    H.find tbl ident
+  with
+    Not_found ->
+      begin
+        if !COption.verbosity > 0 then
+          Format.fprintf fmt warn ident ;
+        H.add tbl ident default ;
+        default
+      end
+
+let find = find_impl registry null_checker "Warning: Checker not found for '%s'. Using null checker.@."
+let find_sol = find_impl sol_registry null_sol_checker "Warning: Solution checker not found for '%s'.@."
 
